sketch runsToSatisfying Inductive Prop, to be used instead of exists fuel, ..., which is much easier to use in proofs with conlusions of the form exists fuel, ...
also, verification revealed a bug in the compilation of OEq and OLt: they override their args if the arg registers alias with the dest register

src/FlatToRiscv.v
@@ -135,14 +135,52 @@ Section FlatToRiscv.
     t = (a, b) -> a = fst t /\ b = snd t.
   Proof. intros. destruct t. inversionss. auto. Qed.
 
+  (* alternative way of saying "exists fuel, run fuel initial = final /\ P final" *)
+  Inductive runsToSatisfying(initial: @RiscvMachine w var)(P: @RiscvMachine w var -> Prop): Prop :=
+    | runsToDone:
+       P initial ->
+       runsToSatisfying initial P
+    | runsToStep:
+       runsToSatisfying (execState run1 initial) P ->
+       runsToSatisfying initial P.
+
+(*
+  (* alternative way of saying "exists fuel, run fuel initial = final /\ P final" *)
+  Inductive runsToSatisfying(P: @RiscvMachine w var -> Prop)(initial: @RiscvMachine w var): Prop :=
+    | runsToDone:
+       P initial ->
+       runsToSatisfying P initial
+    | runsToStep:
+       runsToSatisfying P (execState run1 initial) ->
+       runsToSatisfying P initial.
+
+  (* alternative way of saying "exists fuel, run fuel initial = final /\ P final" *)
+  Inductive runsToSatisfying(P: @RiscvMachine w var -> Prop):
+    forall (initial: @RiscvMachine w var), Prop :=
+    | runsToDone: forall initial,
+       P initial ->
+       runsToSatisfying P initial
+    | runsToStep: forall initial, 
+       runsToSatisfying P (execState run1 initial) ->
+       runsToSatisfying P initial.
+
+  (* alternative way of saying "exists fuel, run fuel initial = final /\ P final" *)
+  Inductive runsToSatisfying:
+    forall (initial: @RiscvMachine w var) (P: @RiscvMachine w var -> Type), Type :=
+    | runsToDone: forall initial P,
+       P initial ->
+       runsToSatisfying initial P
+    | runsToStep: forall initial P, 
+       runsToSatisfying (execState run1 initial) P ->
+       runsToSatisfying initial P.
+*)
+
   Lemma compile_stmt_correct_aux: forall fuelH s insts initialH finalH initialL,
     compile_stmt s = insts ->
     eval_stmt fuelH initialH s = Success finalH ->
     containsProgram initialL insts initialL.(pc) ->
     containsState initialL initialH ->
-    exists (fuelL: nat) (finalL: RiscvMachine),
-      execState (run fuelL) initialL = finalL /\
-      containsState finalL finalH.
+    runsToSatisfying initialL (fun finalL => containsState finalL finalH).
   Proof.
     induction fuelH; [intros; discriminate |].
     introv C EvH Cp Cs.
@@ -150,53 +188,52 @@ Section FlatToRiscv.
     - subst.
       apply containsProgram_cons_inv in Cp. apply proj1 in Cp.
       destruct initialL as [initialProg initialRegs initialPc].
-      exists 1. eexists. simpl.
-      split.
-      + cbv [execState StateMonad.put execute instructionMem registers pc].
-        simpl in Cp.
-        rewrite Cp. simpl. reflexivity.
-      + eapply containsState_put; [eassumption|].
-        (* TODO holds if we add the right assumptions *) admit.
+      apply runsToStep. apply runsToDone.
+      cbv [execState run1 StateMonad.put execute instructionMem registers pc].
+      simpl.
+      simpl in Cp.
+      rewrite Cp. simpl.
+      eapply containsState_put; [eassumption|].
+      (* TODO holds if we add the right assumptions *) admit.
     - simpl in C. subst.
       destruct initialL as [initialProg initialRegs initialPc].
       simpl in Cp.
+      pose proof Cs as Cs'.
       unfold containsState in Cs. simpl in Cs.
       rename H into Gy, H0 into Gz. apply Cs in Gy. apply Cs in Gz.
       subst x0 x1.
-      destruct op;
-      lazymatch goal with
-      | Cp: containsProgram ?s ?p ?PC |- _ =>
-        let p' := eval simpl in p in
-        change (containsProgram s p' PC) in Cp;
-        let l := eval cbv in (length p') in exists l;
-        eexists; (split;
-        [ cbv [run execState StateMonad.put execute instructionMem registers 
+      apply runsToStep.
+      cbv [run1 execState StateMonad.put execute instructionMem registers 
                pc getPC loadInst setPC getRegister setRegister myRiscvMachine IsRiscvMachine gets
-               StateMonad.get Return Bind State_Monad ];
-          repeat (
-            apply containsProgram_cons_inv in Cp;
-            let Cp' := fresh Cp in 
-            destruct Cp as [Cp' Cp];
-            simpl in Cp'
-          );
-          repeat match goal with
-          | E: ?t = ?rhs |- context [?t] => rewrite E
-          end;
-          simpl;
-          lazymatch goal with
-          | |- mkRiscvMachine _ _ _ = _ => reflexivity
-          | |- _ => idtac
-          end
-        | try (unify l 1; eapply containsState_put; [eassumption|reflexivity]) ])
-      end.
-      { assert (initialRegs R0 ^+ initialRegs R0 = $0) as ER0 by admit. (* TODO *)
+               StateMonad.get Return Bind State_Monad ].
+      destruct op;
+      repeat (
+        apply containsProgram_cons_inv in Cp;
+        let Cp' := fresh Cp in 
+        destruct Cp as [Cp' Cp];
+        simpl in Cp'
+      );
+      repeat match goal with
+      | E: ?t = ?rhs |- context [?t] => rewrite E
+      end;
+      simpl;
+      try (apply runsToDone; eapply containsState_put; [eassumption|reflexivity]).
+      + apply runsToStep.
+        cbv [run1 execState StateMonad.put execute instructionMem registers 
+               pc getPC loadInst setPC getRegister setRegister myRiscvMachine IsRiscvMachine gets
+               StateMonad.get Return Bind State_Monad ].
+        rewrite Cp1. simpl.
+        assert (initialRegs R0 ^+ initialRegs R0 = $0) as ER0 by admit. (* TODO *)
         rewrite ER0.
         match goal with
         | |- context [weq ?a ?b] => destruct (weq a b) eqn: E
         end.
-        - rewrite Cp2. simpl. reflexivity.
-        - (* problem: here we should only have made 2 steps instead of 3 *)
-
+        * apply runsToStep.
+          cbv [run1 execState StateMonad.put execute instructionMem registers 
+               pc getPC loadInst setPC getRegister setRegister myRiscvMachine IsRiscvMachine gets
+               StateMonad.get Return Bind State_Monad ]. simpl.
+          rewrite Cp2. simpl.
+          apply runsToDone.
 
   Abort.
 
